tactic stuff again

src/computational_monads/distribution_semantics/tactics.lean
@@ -3,7 +3,8 @@ Copyright (c) 2023 Devon Tuma. All rights reserved.
 Released under Apache 2.0 license as described in the file LICENSE.
 Authors: Devon Tuma
 -/
-import computational_monads.distribution_semantics.monad
+import computational_monads.distribution_semantics.return
+import computational_monads.distribution_semantics.bind
 
 /-!
 # Induction Tactics for Distribution Semantics of `oracle_comp`
@@ -11,26 +12,48 @@ import computational_monads.distribution_semantics.monad
 This file defines custom tactics for working with and proving instances of `dist_equiv`.
 -/
 
-open interactive interactive.types tactic
+open interactive interactive.types
 
 variables {α β γ : Type} {spec : oracle_spec}
 
-namespace tactic.interactive.oracle_comp
+/-- Tag for lemmas to be automatically applied by `pairwise_dist_equiv`. -/
+meta def simp_dist_equiv : user_attribute :=
+{ name := "simp_dist_equiv",
+  descr := "Lemmas tagged with this attribute are automatically called by the
+              `pairwise_dist_equiv` tactic, similar to the way the `simp` tactic works." }
 
-private meta def rw_dist_equiv_base (d_eq : expr) : tactic bool :=
-tactic.apply d_eq >> return tt <|>
-  tactic.refine ``(symm _) >> tactic.apply d_eq >> return tt <|>
-    return ff
+run_cmd attribute.register "simp_dist_equiv"
 
-/-- Attempt to discharge a distributional equivalence between two computations,
-using both definitional equality and the lemmas in the provided list.
-Unsolved goals are pushed to the bottom of the goal list.
-TODO: this could behave weirdly if `rw_dist_equiv_base` somehow discharges two goals. -/
-private meta def pairwise_dist_equiv_base (d_eqs : list pexpr) : tactic unit :=
-do `(%%oa ≃ₚ %%oa') ← tactic.target <|> tactic.fail ("Goal must be a distributional equivalence"),
-  (tactic.unify oa oa' >> tactic.congr) <|> -- Try to solve by unifying terms on each side.
-    (d_eqs.mmap (λ d, tactic.to_expr d >>= rw_dist_equiv_base) >>=
-      λ bs, if tt ∉ bs then tactic.rotate 1 else return ()) -- Rotate if not discharged.
+private meta def get_simp_dist_equiv_lemmas : tactic (list pexpr) :=
+do {tagged_d_eqs ← (attribute.get_instances "simp_dist_equiv"),
+  t' ← mmap tactic.get_decl tagged_d_eqs,
+  d ←  return (list.map declaration.value t'),
+  q ← return (list.map pexpr.of_expr d),
+  return q
+}
+
+namespace oracle_comp
+
+/-- Discharge a distributional equivalence between definitionally equal computations.-/
+private meta def refl_dist_equiv_base : tactic unit :=
+do `(%%oa ≃ₚ %%oa') ← tactic.target, (tactic.unify oa oa' >> tactic.reflexivity)
+
+/-- Attempt to discharge the current goal using the given lemma (potentially in reverse).
+Returns a boolean representing success or failure -/
+private meta def rw_dist_equiv_base (d_eq : expr) : tactic unit :=
+(tactic.apply d_eq >> return ()) <|>
+  (tactic.refine ``(symm _) >> tactic.apply d_eq >> return ())
+
+/-- Given a list of distributional equivalences, call `rw_dist_equiv_base` until one succeeds.
+Immediately stops if the current goal is discharged. -/
+private meta def apply_dist_equivs : list pexpr → tactic unit
+| [] := tactic.rotate 1 -- If the goal is never solved then rotate it to the last goal.
+| (d_eq :: d_eqs) := tactic.to_expr d_eq >>= rw_dist_equiv_base <|>
+                      apply_dist_equivs d_eqs
+
+-- do
+--     (d_eqs.mmap (λ d, tactic.to_expr d >>= rw_dist_equiv_base) >>=
+--       λ bs, if tt ∉ bs then tactic.rotate 1 else return ()) -- Rotate if not discharged.
 
 /-- Destruct a distributional equivalence by recursively splitting equivalences between binds
 into multiple equivalences between their individual components.
@@ -39,7 +62,7 @@ private meta def destruct_pairwise_dist_equiv (d_eq : list pexpr) : expr → tac
 | `(%%oa >>= %%ob ≃ₚ %%oa' >>= %%ob') := do {
   -- Check that the first components of each bind operation have the same type.
   `(oracle_comp %%spec %%α) ← tactic.infer_type oa,
-  `(oracle_comp %%spec %%α') ← tactic.infer_type oa',
+  `(oracle_comp %%spec' %%α') ← tactic.infer_type oa',
   tactic.unify α α', -- Will exit to the `pairwise_dist_equiv_base` below on failure.
   -- Split the goal into two seperate distributional equivalences.
   tactic.refine ``(oracle_comp.bind_dist_equiv_bind_of_dist_equiv _ _),
@@ -48,16 +71,43 @@ private meta def destruct_pairwise_dist_equiv (d_eq : list pexpr) : expr → tac
   -- Attempt to recursively solve the second equivalence
   tactic.intros >> tactic.target >>= destruct_pairwise_dist_equiv
   -- On failure, try to solve the equivalence without any recursion.
-} <|> pairwise_dist_equiv_base d_eq
-| _ := pairwise_dist_equiv_base d_eq
+} <|> refl_dist_equiv_base <|> apply_dist_equivs d_eq
+| _ := refl_dist_equiv_base <|> apply_dist_equivs d_eq
 
-/-- Tactic for reducing proofs of distributional equivalences between bind operations
-into pairwise proofs of equivalences between each component.
-Attempts to discharge trivial goals using both `congr` and the given equivalences. -/
-meta def pairwise_dist_equiv (opt_d_eqs : parse (optional (pexpr_list))) : tactic unit :=
-tactic.target >>= destruct_pairwise_dist_equiv (opt_d_eqs.get_or_else [])
+/-- Tactic for reducing proofs of distributional equivalences between bind operations.
+This introduces goals for pairwise proofs of equivalences between each component.
+Attempts to discharge trivial goals using both `refl` and the given equivalences.
+Supports `dist_equiv`, `eval_dist`, `prob_event`, `support`, and `fin_support`,
+in each case trying to prove the goal by first proving a distributional equivalence. -/
+@[interactive] meta def pairwise_dist_equiv (opt_d_eqs : parse (optional (pexpr_list))) :=
+do g ← tactic.target,
+  passed_d_eqs ← return (opt_d_eqs.get_or_else []),
+  tagged_d_eqs ← get_simp_dist_equiv_lemmas,
+  d_eqs ← return (passed_d_eqs ++ tagged_d_eqs),
+match g with
+-- If the target is a distributional equivalence, begin solving it immedeately.
+| `(%%oa ≃ₚ %%oa') := destruct_pairwise_dist_equiv d_eqs g
+-- If the target is an equality between `eval_dist`s, convert to equivalence notation first.
+| `(⁅%%oa⁆ = ⁅%%oa'⁆) := tactic.refine ``(oracle_comp.dist_equiv.def.1 _) >>
+    tactic.target >>= destruct_pairwise_dist_equiv d_eqs
+-- If the target is an equality between `prob_event`s, switch to equivalence first
+| `(⁅%%e | %%oa⁆ = ⁅%%e' | %%oa'⁆) :=
+    tactic.unify e e' >> tactic.refine ``(oracle_comp.dist_equiv.prob_event_eq _ %%e) >>
+      tactic.target >>= destruct_pairwise_dist_equiv d_eqs <|>
+    tactic.refine ``(oracle_comp.dist_equiv.prob_event_eq_of_inter_support_eq _ _) >>
+      tactic.target >>= destruct_pairwise_dist_equiv d_eqs
+-- If the target is an equality between `support`s, switch to equivalence first
+| `(oracle_comp.support %%oa = oracle_comp.support %%oa') :=
+    tactic.refine ``(oracle_comp.dist_equiv.support_eq _) >>
+      tactic.target >>= destruct_pairwise_dist_equiv d_eqs
+-- If the target is an equality between `fin_support`s, switch to equivalence first
+| `(oracle_comp.fin_support %%oa = oracle_comp.fin_support %%oa') :=
+    tactic.refine ``(oracle_comp.dist_equiv.fin_support_eq _) >>
+      tactic.target >>= destruct_pairwise_dist_equiv d_eqs
+| _ := tactic.fail "Goal must be a distributional equivalence"
+end
 
-end tactic.interactive.oracle_comp
+end oracle_comp
 
 section tests
 
@@ -65,12 +115,32 @@ section tests
 and automatically discharge goals that have provided equivalences or definitional equality. -/
 example (oa oa' : oracle_comp spec α) (ob : α → oracle_comp spec β)
   (h : oa ≃ₚ oa') : (oa >>= ob) ≃ₚ (oa' >>= ob) :=
-by oracle_comp.pairwise_dist_equiv [h]
+by pairwise_dist_equiv [h]
+
+/-- `pairwise_dist_equiv` should work on `eval_dist`. -/
+example (oa oa' : oracle_comp spec α) (ob : α → oracle_comp spec β)
+  (h : oa ≃ₚ oa') : ⁅oa >>= ob⁆ = ⁅oa' >>= ob⁆ :=
+by pairwise_dist_equiv [h]
+
+/-- `pairwise_dist_equiv` should work on `prob_event`. -/
+example (oa oa' : oracle_comp spec α) (ob : α → oracle_comp spec β) (e e' : set β) (h' : oa ≃ₚ oa')
+  (h : e ∩ (oa >>= ob).support = e' ∩ (oa >>= ob).support) : ⁅e | oa >>= ob⁆ = ⁅e' | oa' >>= ob⁆ :=
+by {pairwise_dist_equiv [h'], exact h}
+
+/-- `pairwise_dist_equiv` should work on `support`. -/
+example (oa oa' : oracle_comp spec α) (ob : α → oracle_comp spec β)
+  (h : oa ≃ₚ oa') : (oa >>= ob).support = (oa' >>= ob).support :=
+by pairwise_dist_equiv [h]
+
+/-- `pairwise_dist_equiv` should work on `fin_support`. -/
+example (oa oa' : oracle_comp spec α) (ob : α → oracle_comp spec β)
+  (h : oa ≃ₚ oa') : (oa >>= ob).fin_support = (oa' >>= ob).fin_support :=
+by pairwise_dist_equiv [h]
 
 /-- `pairwise_dist_equiv` should be able to apply given equivalences in reverse as well. -/
 example (oa oa' : oracle_comp spec α) (ob : α → oracle_comp spec β)
   (h : oa ≃ₚ oa') : (oa' >>= ob) ≃ₚ (oa >>= ob) :=
-by oracle_comp.pairwise_dist_equiv [h]
+by pairwise_dist_equiv [h]
 
 /-- `pairwise_dist_equiv` should leave extra goals for equivalences it can't solve-/
 example (oa oa' : oracle_comp spec α) (ob ob' : α → oracle_comp spec β)
@@ -78,8 +148,8 @@ example (oa oa' : oracle_comp spec α) (ob ob' : α → oracle_comp spec β)
   (h : oa ≃ₚ oa') (h' : ∀ a, ob a ≃ₚ ob' a) (h'' : ∀ a b, oc a b ≃ₚ oc' a b) :
   ((oa >>= f) >>= λ x, ob x >>= λ y, oc x y) ≃ₚ ((oa' >>= f) >>= λ x, ob' x >>= λ y, oc' x y) :=
 begin
-  oracle_comp.pairwise_dist_equiv,
-  apply h, apply h', apply h''
+  pairwise_dist_equiv [],
+  apply h, apply h', apply h'',
 end
 
 /-- If two bind operations have mismatched intermediate types, but there is an existing equivalence
@@ -87,7 +157,7 @@ between the two, then `pairwise_dist_equiv` should be able to solve without erro
 example (oa : oracle_comp spec α) (oa' : oracle_comp spec γ)
   (ob : α → oracle_comp spec β) (ob' : γ → oracle_comp spec β)
   (h : oa >>= ob ≃ₚ oa' >>= ob') : oa >>= ob ≃ₚ oa' >>= ob' :=
-by oracle_comp.pairwise_dist_equiv [h]
+by pairwise_dist_equiv [h]
 
 /-- `pairwise_dist_equiv` should be able to handle nested branching of binding operations,
 as well as equivalence arguments with many parameters -/
@@ -96,12 +166,12 @@ example (oa oa' : oracle_comp spec α) (hoa : oa ≃ₚ oa')
   (oc oc' : α → β → oracle_comp spec α) (hoc : ∀ a b, oc a b ≃ₚ oc' a b) :
   ((oa' >>= λ x, ob x >>= λ y, oc x y) >>= λ x, ob x >>= λ y, oc' x y) ≃ₚ
     ((oa >>= λ x, ob' x >>= λ y, oc' x y) >>= λ x, ob' x >>= λ y, oc' x y) :=
-by oracle_comp.pairwise_dist_equiv [hoa, hob, hoc]
+by pairwise_dist_equiv [hoa, hob, hoc]
 
 /-- `pairwise_dist_equiv` can do non-syntactical equality checking. -/
 example (oa oa' : ℕ → oracle_comp spec α) (h : ∀ n, oa n ≃ₚ oa' n):
   (do {x ← return 6, y ← oa x, return 5} : oracle_comp spec ℕ) ≃ₚ
   (do {x ← return (1 * 2 * 3), y ← oa' x, return (10 - 3 - 2)} : oracle_comp spec ℕ) :=
-by oracle_comp.pairwise_dist_equiv [h]
+by pairwise_dist_equiv [h]
 
 end tests
