src/computational_monads/distribution_semantics/monad.lean
@@ -3,8 +3,7 @@ Copyright (c) 2023 Devon Tuma. All rights reserved.
 Released under Apache 2.0 license as described in the file LICENSE.
 Authors: Devon Tuma
 -/
-import computational_monads.distribution_semantics.return
-import computational_monads.distribution_semantics.bind
+import computational_monads.distribution_semantics.tactics
 
 /-!
 # Probability Distributions of Monadic Oracle Constructions
@@ -23,36 +22,31 @@ section return_bind
 
 variables (a : α) (ob : α → oracle_comp spec β) (y : β) (e' : set β)
 
-lemma support_return_bind : (return a >>= ob).support = (ob a).support :=
-by simp only [support_bind, mem_support_return_iff, set.Union_Union_eq_left]
-
-lemma mem_support_return_bind_iff : y ∈ (return a >>= ob).support ↔ y ∈ (ob a).support :=
-by rw [support_return_bind]
-
-lemma fin_support_return_bind : (return a >>= ob).fin_support = (ob a).fin_support :=
-by simp only [fin_support_bind, fin_support_return, finset.singleton_bUnion]
-
-lemma mem_fin_support_return_bind_iff :
-  y ∈ (return a >>= ob).fin_support ↔ y ∈ (ob a).fin_support :=
-by rw [fin_support_return_bind]
-
-lemma return_bind_dist_equiv : return a >>= ob ≃ₚ ob a :=
+@[simp_dist_equiv] lemma return_bind_dist_equiv : return a >>= ob ≃ₚ ob a :=
 by simp only [dist_equiv.def, eval_dist_bind, eval_dist_return, pmf.pure_bind]
 
+lemma support_return_bind : (return a >>= ob).support = (ob a).support :=
+by pairwise_dist_equiv
+
+lemma fin_support_return_bind : (return a >>= ob).fin_support = (ob a).fin_support :=
+by pairwise_dist_equiv
+
 lemma eval_dist_return_bind : ⁅return a >>= ob⁆ = ⁅ob a⁆ :=
-(return_bind_dist_equiv a ob).eval_dist_eq
+by pairwise_dist_equiv
 
 lemma eval_dist_return_bind_apply : ⁅= y | return a >>= ob⁆ = ⁅= y | ob a⁆ :=
 (return_bind_dist_equiv a ob).eval_dist_apply_eq y
 
 @[simp] lemma prob_event_return_bind : ⁅e' | return a >>= ob⁆ = ⁅e' | ob a⁆ :=
-(return_bind_dist_equiv a ob).prob_event_eq e'
+by pairwise_dist_equiv
 
 end return_bind
 
 section bind_return
 
 variables (oa : oracle_comp spec α) (f : α → β) (y : β) (e' : set β)
+
+section support
 
 @[simp] lemma support_bind_return : (oa >>= λ x, return (f x)).support = f '' oa.support :=
 calc (oa >>= λ x, return (f x)).support = ⋃ x ∈ oa.support, {f x} : rfl
@@ -72,27 +66,25 @@ lemma mem_fin_support_bind_return_iff [decidable_eq β] :
   y ∈ (oa >>= λ a, return (f a)).fin_support ↔ ∃ x ∈ oa.fin_support, f x = y :=
 by simp only [fin_support_bind_return, finset.mem_image]
 
+end support
+
+section eval_dist
+
 @[simp] lemma eval_dist_bind_return : ⁅oa >>= λ x, return (f x)⁆ = ⁅oa⁆.map f :=
 by simp_rw [eval_dist_bind, eval_dist_return, pmf.bind_pure_comp]
-
 
 lemma eval_dist_bind_return_apply_eq_tsum [decidable_eq β] :
   ⁅oa >>= λ x, return (f x)⁆ y = ∑' x, ite (y = f x) (⁅oa⁆ x) 0 :=
 begin
   rw [eval_dist_bind_return, pmf.map_apply],
-  congr,
-  refine funext (λ x, _),
-  congr,
+  refine tsum_congr (λ x, by congr)
 end
 
--- TODO: gross proof
 lemma eval_dist_bind_return_apply_eq_tsum_indicator :
   ⁅oa >>= λ x, return (f x)⁆ y = ∑' x, (f ⁻¹' {y}).indicator ⁅oa⁆ x :=
 begin
-  rw [eval_dist_bind_apply_eq_tsum],
-  refine tsum_congr (λ x, _),
-  rw [eval_dist_return, pmf.pure_apply, set.indicator],
-  rw [mul_ite, mul_one, mul_zero, @eq_comm _ y],
+  refine (eval_dist_bind_apply_eq_tsum _ _ _).trans (tsum_congr $ λ x, _),
+  rw [eval_dist_return, pmf.pure_apply, set.indicator, mul_ite, mul_one, mul_zero, @eq_comm _ y],
   congr,
 end
 
@@ -117,11 +109,17 @@ lemma eval_dist_bind_return_apply_eq_sum_fin_support_indicator :
   (tsum_eq_sum (λ x hx, by simp_rw [set.indicator_apply_eq_zero,
     eval_dist_eq_zero_iff', hx, not_false_iff, imp_true_iff]))
 
+end eval_dist
+
+section prob_event
+
 @[simp] lemma prob_event_bind_return : ⁅e' | oa >>= λ a, return (f a)⁆ = ⁅f ⁻¹' e' | oa⁆ :=
 begin
   rw [prob_event_bind_eq_tsum, prob_event_eq_tsum_indicator],
   refine tsum_congr (λ x, by simpa only [prob_event_return_eq_indicator, set.indicator, mul_boole])
 end
+
+end prob_event
 
 end bind_return
 
@@ -129,21 +127,19 @@ section bind_return_id
 
 variables (oa : oracle_comp spec α) (y : β) (e' : set β)
 
-@[simp] lemma support_bind_return_id : (oa >>= return).support = oa.support :=
-(support_bind_return oa id).trans (set.image_id oa.support)
-
-@[simp] lemma fin_support_bind_return_id [decidable_eq α] :
-  (oa >>= return).fin_support = oa.fin_support :=
-(fin_support_bind_return oa id).trans finset.image_id
-
-lemma bind_return_id_dist_equiv : oa >>= return ≃ₚ oa :=
+@[simp_dist_equiv] lemma bind_return_id_dist_equiv : oa >>= return ≃ₚ oa :=
 (eval_dist_bind_return oa id).trans (by rw [pmf.map_id])
 
-@[simp] lemma eval_dist_bind_return_id : ⁅oa >>= return⁆ = ⁅oa⁆ :=
-(bind_return_id_dist_equiv oa).eval_dist_eq
+@[simp] lemma support_bind_return_id : (oa >>= return).support = oa.support :=
+by pairwise_dist_equiv
+
+@[simp] lemma fin_support_bind_return_id [decidable_eq α] :
+  (oa >>= return).fin_support = oa.fin_support := by pairwise_dist_equiv
+
+@[simp] lemma eval_dist_bind_return_id : ⁅oa >>= return⁆ = ⁅oa⁆ := by pairwise_dist_equiv
 
 @[simp] lemma prob_event_bind_return_id (e : set α) : ⁅e | oa >>= return⁆ = ⁅e | oa⁆ :=
-by rw [prob_event_bind_return, set.preimage_id']
+by pairwise_dist_equiv
 
 end bind_return_id
 
