src/computational_monads/simulation_semantics/is_stateless.lean
@@ -46,7 +46,7 @@ instance is_stateless.is_tracking [hso : so.is_stateless] : so.is_tracking :=
     begin
       sorry,
       -- refine λ i t s, trans ((eval_dist_map_id $ (so i (t, s))).symm.trans
-      --   (map_equiv_congr (λ x, _) (by rw so.state_elim s))) (eval_dist_map_comp' _ _ _).symm,
+      --   (map_equiv_congr (λ x, _) (by rw so.state_elim s))) (eval_dist_map_comp _ _ _).symm,
       -- simp only [prod.eq_iff_fst_eq_snd_eq, so.state_elim x.2, id.def, eq_self_iff_true, and_self]
     end
 }
